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1 Definition

(from Tibsirani, ESL)

2 3 knot splines

We have N1 and N2 from the definition, but we need N3 for a 3 knot spline.

N3 = N1+2(X) = d1(X)− d3−1(X)

where ξk is the location of the kth knot and

d1(X) =
(X − ξ1)

3
+ − (X − ξ3)

3
+

ξ3 − ξ1

and

d2(X) =
(X − ξ2)

3
+ − (X − ξ3)

3
+

ξ3 − ξ2
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so

N3 = N1+2(X) =
(X − ξ1)

3
+ − (X − ξ3)

3
+

ξ3 − ξ1
−

(X − ξ2)
3
+ − (X − ξ3)

3
+

ξ3 − ξ2

and we simplify that.

2.1 Simplify

1. Multiply terms by 1

N3 =
ξ3 − ξ2
ξ3 − ξ2

∗
(X − ξ1)

3
+ − (X − ξ3)

3
+

ξ3 − ξ1
− ξ3 − ξ1

ξ3 − ξ1
∗
(X − ξ2)

3
+ − (X − ξ3)

3
+

ξ3 − ξ2

2. Distribute

=
[(ξ3 − ξ2) ∗ ((X − ξ1)

3
+ − (X − ξ3)

3
+)]− [(ξ3 − ξ1) ∗ ((X − ξ2)

3
+ − (X − ξ3)

3
+)]

(ξ3 − ξ1) ∗ (ξ3 − ξ2)

=
[(ξ3 − ξ2) ∗ (X − ξ1)

3
+ − (ξ3 − ξ2) ∗ (X − ξ3)

3
+]− [(ξ3 − ξ1) ∗ (X − ξ2)

3
+ − (ξ3 − ξ1) ∗ (X − ξ3)

3
+]

(ξ3 − ξ1) ∗ (ξ3 − ξ2)

3. Cancel and simplify

=
(ξ3 − ξ2) ∗ (X − ξ1)

3
+ − (ξ3 − ξ2) ∗ (X − ξ3)

3
+ − (ξ3 − ξ1) ∗ (X − ξ2)

3
+ + (ξ3 − ξ1) ∗ (X − ξ3)

3
+

(ξ3 − ξ1) ∗ (ξ3 − ξ2)

=
(ξ3 − ξ2) ∗ (X − ξ1)

3
+ − (ξ3 − ξ1) ∗ (X − ξ2)

3
+ [−(ξ3 − ξ2) + (ξ3 − ξ1)] ∗ (X − ξ3)

3
+

(ξ3 − ξ1) ∗ (ξ3 − ξ2)

=
(ξ3 − ξ2) ∗ (X − ξ1)

3
+ − (ξ3 − ξ1) ∗ (X − ξ2)

3
+ + (ξ2 − ξ1) ∗ (X − ξ3)

3
+

(ξ3 − ξ1) ∗ (ξ3 − ξ2)

4. Divide by 1

=
(ξ3 − ξ2) ∗ (X − ξ1)

3
+ − (ξ3 − ξ1) ∗ (X − ξ2)

3
+ + (ξ2 − ξ1) ∗ (X − ξ3)

3
+

(ξ3 − ξ1) ∗ (ξ3 − ξ2)
÷ (ξ3 − ξ2)

(ξ3 − ξ2)

=
(X − ξ1)

3
+ −

[
(ξ3−ξ1)
(ξ3−ξ2)

∗ (X − ξ2)
3
+

]
+

[
(ξ2−ξ1)
(ξ3−ξ2)

∗ (X − ξ3)
3
+

]
(ξ3 − ξ1)
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